# 4ï¸âƒ£ Sum Rule

## ğŸ”¹ Big Idea

The derivative of a sum is the sum of the derivatives.

If:

f(x) = g(x) + h(x)

Then:

d/dx [ g(x) + h(x) ] = g'(x) + h'(x)

---

## ğŸ§  What Does This Mean?

Instead of differentiating the whole expression at once:

We differentiate each part separately.

Then add the results.

---

## ğŸ§  Simple Example

Let:

f(x) = xÂ² + xÂ³

Using power rule:

d/dx (xÂ²) = 2x  
d/dx (xÂ³) = 3xÂ²  

So:

f'(x) = 2x + 3xÂ²

---

## ğŸ§  Another Example

f(x) = xâ´ + x + 7

Derivative of each term:

d/dx (xâ´) = 4xÂ³  
d/dx (x) = 1  
d/dx (7) = 0  

So:

f'(x) = 4xÂ³ + 1 + 0

Final Answer:

f'(x) = 4xÂ³ + 1

---

## ğŸ§  More Example

f(x) = 5xÂ² + 3xÂ³ + 10

Step 1: Differentiate each term

d/dx (5xÂ²) = 10x  
d/dx (3xÂ³) = 9xÂ²  
d/dx (10) = 0  

Step 2: Add them

f'(x) = 10x + 9xÂ²

---

## ğŸ§  Important Pattern

Original Function:

xÂ² + xÂ³ + xâ´

Derivative:

2x + 3xÂ² + 4xÂ³

Each term is treated independently.

---

## ğŸ¤– Why Sum Rule Matters in Deep Learning

Neural network loss functions often look like:

Loss = (prediction âˆ’ target)Â² + regularization_term

To compute gradient:

We take derivative of each part separately.

Then add them.

Without sum rule, backpropagation would not work cleanly.

Sum rule allows:

âœ” Breaking complex expressions  
âœ” Computing gradients term by term  
âœ” Building large models easily  

---

## ğŸ§© Intuition Summary

Derivative of:

A + B + C

Equals:

Derivative of A  
+ Derivative of B  
+ Derivative of C  

Just differentiate each term and add.

---

## ğŸ”¹ Practice Questions

1. d/dx (xÂ³ + xÂ²) = ?  
2. d/dx (xâµ + x + 4) = ?  
3. d/dx (xâ´ + 7) = ?  

Answers:

1. 3xÂ² + 2x  
2. 5xâ´ + 1  
3. 4xÂ³  