\# 6ï¸âƒ£ Chain Rule



\## ğŸ”¹ Big Idea



The Chain Rule is used when a function is inside another function.



If:



f(x) = g(h(x))



Then:



f'(x) = g'(h(x)) Â· h'(x)



In simple words:



Derivative of outer function  

Ã—  

Derivative of inner function



---



\## ğŸ§  Why Do We Need Chain Rule?



Sometimes functions are nested.



Example:



f(x) = (xÂ² + 3)Â²



Here:



Outer function: somethingÂ²  

Inner function: xÂ² + 3  



We cannot use power rule directly.



We must use Chain Rule.



---



\## ğŸ§  Step-by-Step Method



When you see:



(something)^n



Follow these steps:



1\. Differentiate the outer power  

2\. Keep the inside unchanged  

3\. Multiply by derivative of inside  



---



\## ğŸ§  Example 1



f(x) = (xÂ² + 3)Â²



Step 1: Differentiate outer function



2(xÂ² + 3)



Step 2: Multiply by derivative of inside



Derivative of (xÂ² + 3) = 2x



Step 3: Multiply everything



f'(x) = 2(xÂ² + 3) Â· 2x



Final Answer:



f'(x) = 4x(xÂ² + 3)



---



\## ğŸ§  Example 2



f(x) = (3x + 1)â´



Step 1: Derivative of outer power



= 4(3x + 1)Â³



Step 2: Derivative of inside



= 3



Step 3: Multiply



f'(x) = 4(3x + 1)Â³ Â· 3



Final Answer:



f'(x) = 12(3x + 1)Â³



---



\## ğŸ§  Example 3



f(x) = âˆš(xÂ² + 1)



Rewrite first:



f(x) = (xÂ² + 1)^(1/2)



Step 1: Derivative of outer power



= (1/2)(xÂ² + 1)^(-1/2)



Step 2: Derivative of inside



= 2x



Step 3: Multiply



f'(x) = (1/2)(xÂ² + 1)^(-1/2) Â· 2x



Simplify:



f'(x) = x(xÂ² + 1)^(-1/2)



---



\## ğŸ§  Pattern to Remember



If:



f(x) = (u)^n



Then:



f'(x) = n(u)^(n-1) Â· u'



Where:



u = inner function  

u' = derivative of inner function  



---



\## ğŸ¤– Why Chain Rule Is Extremely Important in Deep Learning



Neural networks are nested functions.



Example:



Loss = L( activation( wx + b ) )



That is:



Function inside function inside function.



Backpropagation uses Chain Rule repeatedly.



Without Chain Rule:



Deep learning cannot work.



Chain Rule = backbone of backpropagation.



---



\## ğŸ§© Intuition Summary



Outer function changes  

Inner function also changes  



Total change =



(outer change) Ã— (inner change)



Chain Rule connects multiple layers of change.



---



\## ğŸ”¹ Practice Questions



1\. d/dx (xÂ² + 5)Â³ = ?  

2\. d/dx (2x + 1)âµ = ?  

3\. d/dx âˆš(3xÂ² + 4) = ?  



Answers:



1\. 3(xÂ² + 5)Â² Â· 2x  

2\. 5(2x + 1)â´ Â· 2  

3\. (1/2)(3xÂ² + 4)^(-1/2) Â· 6x  

